Instructions.v
@@ -2,17 +2,14 @@ Add LoadPath "D:\DVM".
 Require Export Eval.
 Require Export Example.
 Require Export Method.
-<<<<<<< HEAD
 Require Export DType.
-=======
->>>>>>> master
 
 Module Type InstructionType.
   Parameter inst : Type. (* ADT for Instrucion *)
   Parameter mthd : Type. (* ADT for Methods *)
   Parameter prg : Type. (* ADT for Programs*)
   Parameter toEval : inst -> list rhs.
-  Parameter evalNop : DVMState -> prg -> list deltaState.
+  Parameter stepFix : DVMState -> prg -> @Option DVMState.
   (* Parameter evalWith : inst -> DVMState -> list ValOrRef -> list deltaState. *)
 End InstructionType.
 
@@ -31,30 +28,27 @@ Module INSTRUCTION <: InstructionType.
     | branch r1 _ r2 _ => (cons r1 (cons r2 nil))
     | move _ r1 => (cons r1 nil)
     | update r1 r2 => (cons r1 (cons r2 nil))
-<<<<<<< HEAD
     | unary _ _ r1 => (cons r1 nil)
-=======
-    | unaryArith _ _ r1 => (cons r1 nil)
->>>>>>> master
     | binaryArith _ r1 _ r2 => (cons r1 (cons r2 nil))
     | new _ _ => nil
     | newarr _ _ r1 => (cons r1 nil)
     | cast _ _ r1 => (cons r1 nil)
-    | read _ _ => nil
-    | print _ r1 => (cons r1 nil)
+    | read _ => nil
+    | print _ => nil
+    | hlt => nil
     end.
 
-  Definition evalNop (curr:DVMState) (p:prg) : list deltaState :=
+  Definition evalNop (curr:DVMState) (p:prg) : deltaState :=
     match curr with
-    | stuck => [mkStuck]
-    | halt => [mkHalt]
-    | dst nil _ _ _ _ => [mkStuck]
+    | stuck => mkStuck
+    | halt => mkHalt
+    | dst nil _ _ _ _ => mkStuck
     | dst (cons (frm vals ml pc) frem) h sh bin bout => match (METHOD.getMethod ml p) with
       | Some md => match (METHOD.getNextPC pc md) with
-        | Some pc' => [updateFrame (upPC pc')]
-        | _ => [mkStuck]
+        | Some pc' => updateFrame (upPC pc')
+        | _ => mkStuck
         end
-      | _ => [mkStuck]
+      | _ => mkStuck
       end
     end.
 
@@ -64,6 +58,14 @@ Module INSTRUCTION <: InstructionType.
       match (METHOD.getMethod ml p) with
       | Some md => match (METHOD.getNextPC pc md) with
         | Some pc' => [deleteFrame ; updateFrame (upVals 201 x) ; updateFrame (upPC pc')]
+        | _ => [mkStuck]
+        end
+      | _ => [mkStuck]
+      end
+    | None,(dst (cons f1 (cons (frm vals ml pc) frem)) h sh bin bout) => 
+      match (METHOD.getMethod ml p) with
+      | Some md => match (METHOD.getNextPC pc md) with
+        | Some pc' => [deleteFrame ; updateFrame (upPC pc')]
         | _ => [mkStuck]
         end
       | _ => [mkStuck]
@@ -78,6 +80,14 @@ Module INSTRUCTION <: InstructionType.
       match (METHOD.getMethod ml p) with
       | Some md => match (METHOD.getNextPC pc md) with
         | Some pc' => [deleteFrame ; updateFrame (upVals n x) ; updateFrame (upPC pc')]
+        | _ => [mkStuck]
+        end
+      | _ => [mkStuck]
+      end
+    | None,(dst (cons f1 (cons (frm vals ml pc) frem)) h sh bin bout) => 
+      match (METHOD.getMethod ml p) with
+      | Some md => match (METHOD.getNextPC pc md) with
+        | Some pc' => [deleteFrame ; updateFrame (upPC pc')]
         | _ => [mkStuck]
         end
       | _ => [mkStuck]
@@ -118,18 +128,18 @@ Module INSTRUCTION <: InstructionType.
     [updateFrame (upPC pc)].
 
   Definition evalBranch (l1 l2:rhs) (bc:BinaryCompOperator) (pc:ProgramCounter) (curr:DVMState) (p:prg) : list deltaState :=
-    match (EVAL.evalRhs l1 curr),(EVAL.evalRhs l1 curr) with
+    match (EVAL.evalRhs l1 curr),(EVAL.evalRhs l2 curr) with
     | Some (prim p1),Some (prim p2) => match bc with
-      | beq => match ((PType.comp p1 p2)+(PType.comp p2 p1))%nat with
+      | beq => match (plus (PType.comp p1 p2) (PType.comp p2 p1))%nat with
         | 0 => [updateFrame (upPC pc)]
-        | _ => (evalNop curr p)
+        | _ => [evalNop curr p]
         end
       | blt => match (PType.comp p2 p1) with
-        | 0 => (evalNop curr p)
+        | 0 => [evalNop curr p]
         | _ => [updateFrame (upPC pc)]
         end
       | bgt => match (PType.comp p1 p2) with
-        | 0 => (evalNop curr p)
+        | 0 => [evalNop curr p]
         | _ => [updateFrame (upPC pc)]
         end
       end
@@ -139,20 +149,15 @@ Module INSTRUCTION <: InstructionType.
       end
     end.
 
-<<<<<<< HEAD
   Definition evalMove (l1:rhs) (n:Register) (curr:DVMState) (p:prg) : list deltaState :=
-=======
-  Definition move (l1:rhs) (n:Register) (curr:DVMState) (p:prg) : list deltaState :=
->>>>>>> master
     match (EVAL.evalRhs l1 curr) with
-    | Some v1 => [updateFrame (upVals n v1)]
+    | Some v1 => (cons (evalNop curr p) [updateFrame (upVals n v1)] )
     | _ => match curr with
       | halt => [mkHalt]
       | _ => [mkStuck]
       end
     end.
 
-<<<<<<< HEAD
   Declare Module HEAP : ListType with Definition t1 := arrOrObj.
   Declare Module VLIST : ListType with Definition t1 := Val.
   Declare Module FLIST : ListType with Definition t1 := FieldLocation*Val.
@@ -164,7 +169,7 @@ Module INSTRUCTION <: InstructionType.
     | (l (acc r1 r2)),(Some v1),(dst frms h sh inb outb) => match (EVAL.evalReg r1 curr),(EVAL.evalReg r2 curr) with
       | (Some (ref (lRef loc1))),(Some (prim p2)) => match (HEAP.get loc1 h),(PType.toNat p2) with
         | Some (ar (arr n1 vlst)),n2 => match (isle_num n2 n1) with
-          | true => [(upHeap [(loc1,(ar (arr n1 (VLIST.set n2 v1 vlst))))])]
+          | true => cons (evalNop curr p) [(upHeap [(loc1,(ar (arr n1 (VLIST.set n2 v1 vlst))))])]
           | _ => [mkStuck]
           end
         | _,_ => [mkStuck]
@@ -174,7 +179,7 @@ Module INSTRUCTION <: InstructionType.
     | (l (ifield r1 f1)),(Some v1),(dst frms h sh inb outb) => match (EVAL.evalReg r1 curr) with
       | Some (ref (lRef loc1)) => match (HEAP.get loc1 h) with
         | Some (dob (obj c1 c2 lst)) => match (FLIST.find (f1,(ref null)) compFirst lst) with
-          | Some n1 => [upHeap [(loc1,(dob (obj c1 c2 (FLIST.set n1 (f1,v1) lst))))]]
+          | Some n1 => cons (evalNop curr p) [upHeap [(loc1,(dob (obj c1 c2 (FLIST.set n1 (f1,v1) lst))))]]
           | _ => [mkStuck]
           end
         | _ => [mkStuck]
@@ -182,7 +187,7 @@ Module INSTRUCTION <: InstructionType.
       | _ => [mkStuck]
       end
     | (l (sfield f1)),(Some v1),(dst frms h sh inb outb) => match (FLIST.find (f1,(ref null)) compFirst sh) with
-      | Some n1 => [upSHeap (FLIST.set n1 (f1,v1) sh)]
+      | Some n1 => cons (evalNop curr p) [upSHeap (FLIST.set n1 (f1,v1) sh)]
       | _ => [mkStuck]
       end
     | _,_,_ => [mkStuck]
@@ -218,12 +223,14 @@ Module INSTRUCTION <: InstructionType.
       end
     end.
 
+  Declare Module HP : ListType with Definition t1 := arrOrObj.
+
   Definition evalNew (n:Register) (cl:ClassLocation) (curr:DVMState) (p:prg) : list deltaState :=
     match curr with
     | stuck => [mkStuck]
     | halt => [mkHalt]
     | (dst _ h _ _ _) => match (TYPE.createObject p (r (c cl)) h) with
-      | Some (upHeap (cons (lc1,vl1) nil)) => (cons (upHeap (cons (lc1,vl1) nil)) (cons (updateFrame (upVals n (ref (lRef lc1)))) nil) )
+      | Some (addHeap vl1) => cons (evalNop curr p) (cons (addHeap vl1) (cons (updateFrame (upVals n (ref (lRef (HP.len h))))) nil) )
       | _ => [mkStuck]
       end
     end.
@@ -233,8 +240,8 @@ Module INSTRUCTION <: InstructionType.
     | stuck,_ => [mkStuck]
     | halt,_ => [mkHalt]
     | (dst _ h _ _ _),(Some v1) => match (EVAL.evalRhs l curr) with
-      | Some (prim p) => match (TYPE.createArray t (PType.toNat p) h) with
-        | Some (upHeap (cons (lc1,vl1) nil)) => (cons (upHeap (cons (lc1,vl1) nil)) (cons (updateFrame (upVals n (ref (lRef lc1)))) nil) )
+      | Some (prim p1) => match (TYPE.createArray t (PType.toNat p1) h) with
+        | Some (addHeap vl1) => cons (evalNop curr p) (cons (addHeap vl1) (cons (updateFrame (upVals n (ref (lRef (HP.len h))))) nil) )
         | _ => [mkStuck]
         end
       | _ => [mkStuck]
@@ -248,7 +255,7 @@ Module INSTRUCTION <: InstructionType.
     | stuck,_ => [mkStuck]
     | (dst frms h sh inb outb),(Some v1) => match v1 with
       | (ref (lRef loc1)) => match (TYPE.cast p t loc1 h) with
-        | Some (upHeap (cons (l1,ob1) nil)) => (cons (upHeap (cons (l1,ob1) nil)) (cons (updateFrame (upVals n (ref (lRef l1)))) nil))
+        | Some (upHeap (cons (l1,ob1) nil)) => cons (evalNop curr p) (cons (upHeap (cons (l1,ob1) nil)) (cons (updateFrame (upVals n (ref (lRef l1)))) nil))
         | _ => [mkStuck]
         end
       | _ => [mkStuck]
@@ -263,7 +270,7 @@ Module INSTRUCTION <: InstructionType.
     | halt => [mkHalt]
     | stuck => [mkStuck]
     | (dst frms h sh (crs,lst) outb) => match (NLIST.get crs lst) with
-      | Some num => cons (upInc (S crs)) (cons (updateFrame (upVals n (prim (int num)))) nil)
+      | Some num => cons (evalNop curr p) (cons (upInc (S crs)) (cons (updateFrame (upVals n (prim (int num)))) nil))
       | None => [mkStuck]
       end
     end.
@@ -272,10 +279,56 @@ Module INSTRUCTION <: InstructionType.
     match curr,(EVAL.evalRhs r1 curr) with
     | halt,_ => [mkHalt]
     | stuck,_ => [mkStuck]
-    | (dst frms h sh inb (crs,lst)),(Some (prim p1)) => [(upOutc (S crs));(upOutb [(crs,(PType.toNat p1))])]
+    | (dst frms h sh inb (crs,lst)),(Some (prim p1)) => cons (evalNop curr p) [(addOutb (PType.toNat p1))]
     | _,_ => [mkStuck]
     end.
 
-=======
->>>>>>> master
+  Definition evalInst (inst:Instruction) (curr:DVMState) (p:prg) : list deltaState :=
+    match inst with
+    | nop => [evalNop curr p]
+    | ret => evalRet curr p
+    | retTo r1 => evalRetTo curr p r1
+    | invokes lst ml => evalInvokes curr p lst ml
+    | invokei r1 lst ml => evalInvokei curr p lst ml r1
+    | goto pc => evalGoto pc
+    | branch r1 bcmp r2 pc => evalBranch r1 r2 bcmp pc curr p
+    | move r1 r2 => evalMove r2 r1 curr p
+    | update r1 r2 => evalUpdate r1 r2 curr p
+    | unary n1 uop r1 => evalUnary r1 n1 uop curr p
+    | binaryArith n1 r1 binop r2 => evalBinaryArith r1 r2 n1 binop curr p
+    | new n1 cl => evalNew n1 cl curr p
+    | newarr n1 t1 r1 => evalNewArray n1 t1 r1 curr p
+    | cast n1 t1 r1 => evalCast n1 t1 r1 curr p
+    | read n1 => evalRead n1 curr p
+    | print r1 => evalWrite r1 curr p
+    | hlt => [mkHalt]
+    end.
+
+  Definition getCurrInstruction (curr:DVMState) (p:prg) : @Option Instruction :=
+    match curr with
+    | (dst (cons (frm _ ml pc) _) _ _ _ _) => match (METHOD.getMethod ml p) with
+      | Some md => METHOD.getInstAt pc md
+      | None => None
+      end
+    | halt => Some hlt
+    | _ => None
+    end.
+
+  Definition stepFix (curr:DVMState) (p:prg) : @Option DVMState :=
+    match (getCurrInstruction curr p) with
+    | Some ins => (ChangeState.mkChanges curr (evalInst ins curr p))
+    | None => None
+    end.
+
+  Fixpoint multiStepFix (n:nat) (curr:DVMState) (p:prg) : @Option DVMState :=
+    match n with
+    | 0 => (stepFix curr p)
+    | S n' => match (stepFix curr p) with
+      | Some st => (multiStepFix n' st p)
+      | None => None
+      end
+    end.
+
+  Compute (multiStepFix 101 currState p).
+
 End INSTRUCTION.
